Missing instances for WriterT, but some not yet solved. Some comments on OptionT.

Control/Monad/Class/MonadWriter.v
@@ -16,7 +16,13 @@ Class MonadWriter (W : Monoid) (M : Type -> Type) (inst : Monad M) : Type :=
       forall (A : Type) (ma : M A),
         listen (listen ma) =
         fmap (fun '(a, w) => ((a, w), neutr)) (listen ma);
+    listen_bind :
+      forall (A B : Type) (ma : M A) (f : A -> M B),
+        listen (ma >>= f) =
+        listen ma >>= fun '(a, w) => fmap (fun b => (b, w)) (f a)
 }.
+
+Search fmap bind.
 
 Hint Rewrite @listen_pure (*@listen_tell*) @listen_listen : HSLib.
 
